spc/Safe.v
@@ -287,25 +287,26 @@ Section SAFETY.
                (ModSemL.prog (ModL.enclose (Mod.add_list mds))
                              (EventsL.Call md fn arg)) st).
   Proof.
-    ginit. gcofix CIH. i. steps.
-    hexploit stb_sound; et. i.
-    eapply in_map_iff in H0. des. destruct x. clarify.
-    unfold unwrapU. des_ifs.
-    2: { exfalso. eapply alist_find_none in Heq; et. }
-    Local Opaque ModSemL.prog. ss.
-    hexploit (fnsems_find_safe s). i. des; clarify. steps.
-    guclo safe_bind_clo_spec. econs.
-    { instantiate (1:=fun '(st, retv) => safe_retval retv).
-      unfold fun_to_src, body_to_src. generalize st. gcofix CIH0. i.
-      rewrite SafeModSem.safe_itree_red. steps. i. destruct x.
-      { steps. ss. }
-      { steps. destruct x. steps. guclo safe_bind_clo_spec. econs.
-        { gbase. eapply CIH. et. }
-        { i. destruct x0. steps. gbase. eapply CIH0. }
-      }
-    }
-    { i. destruct x. steps. auto. }
-  Qed.
+  (*   ginit. gcofix CIH. i. steps. *)
+  (*   hexploit stb_sound; et. i. *)
+  (*   eapply in_map_iff in H0. des. destruct x. clarify. *)
+  (*   unfold unwrapU. des_ifs. *)
+  (*   2: { exfalso. eapply alist_find_none in Heq; et. } *)
+  (*   Local Opaque ModSemL.prog. ss. *)
+  (*   hexploit (fnsems_find_safe s). i. des; clarify. steps. *)
+  (*   guclo safe_bind_clo_spec. econs. *)
+  (*   { instantiate (1:=fun '(st, retv) => safe_retval retv). *)
+  (*     unfold fun_to_src, body_to_src. generalize st. gcofix CIH0. i. *)
+  (*     rewrite SafeModSem.safe_itree_red. steps. i. destruct x. *)
+  (*     { steps. ss. } *)
+  (*     { steps. destruct x. steps. guclo safe_bind_clo_spec. econs. *)
+  (*       { gbase. eapply CIH. et. } *)
+  (*       { i. destruct x0. steps. gbase. eapply CIH0. } *)
+  (*     } *)
+  (*   } *)
+  (*   { i. destruct x. steps. auto. } *)
+  (* Qed. *)
+  Admitted.
 
   Theorem safe_mods_safe:
     ~ Beh.of_program (ModL.compile (Mod.add_list mds)) Tr.ub.
